src/tls/TLSInfo.fst
@@ -1,19 +1,21 @@
 (*--build-config
 options:--use_hints --fstar_home ../../../FStar --include ../../../FStar/ucontrib/Platform/fst/ --include ../../../FStar/ucontrib/CoreCrypto/fst/ --include ../../../FStar/examples/low-level/crypto/real --include ../../../FStar/examples/low-level/crypto/spartan --include ../../../FStar/examples/low-level/LowCProvider/fst --include ../../../FStar/examples/low-level/crypto --include ../../libs/ffi --include ../../../FStar/ulib/hyperstack --include ideal-flags;
 --*)
-(**
- This module gathers the definitions of shared datatypes, parameters, and predicates for our TLS API.
- Its interface is used by most TLS modules; its implementation is typechecked.
-*)
 module TLSInfo
 
 #set-options "--max_fuel 3 --initial_fuel 3 --max_ifuel 1 --initial_ifuel 1"
 
-open FStar.HyperStack
+(* This module gathers the definitions of
+   public datatypes, parameters, and predicates for our TLS API.
+
+   Its interface is used by most TLS modules;
+   its implementation is typechecked.
+*)
+
 open Platform.Bytes
 open Platform.Date
 open TLSConstants
-open FStar.ST
+//open PMS
 open Cert
 
 module MM = MonotoneMap
@@ -22,25 +24,22 @@ module HH = FStar.HyperHeap
 
 
 (**************** SPECIFYING SAFETY (GENERAL COMMENTS) **************
-  The definition of safety has changed substantially from miTLS 0.9.
-  We record safety of various secret and key indexes in this module
-  as witnesses of being recorded in the monotonic safety table.
+  In the code of ideal implementations only,
+  we use F# functions that characterize the Safe and Auth predicates.
 
-  Safety of all indexes is bootstrapped from the safety of Diffie-Hellman
-  shares, as defined in CommonDH, and pre-shared keys, as defined in PSK.
-  Thus, we enforce by typing that honest derived indexes require that the
-  source index of the derivation is also honest. This is possible because the
-  index structure is fully defined in this module.
+  We need to typecheck ideal code,
+  so we write their modules in the style
 
-  Conversly, the honesty of derived indexes is not fixed by the the honety
-  of the source key material's index: during the derivation, the attacker may
-  request the derived index to be compromised.
+  #if ideal
+    if safe...(...)
+      ... GEN ...
+    else
+  ##endif
+  .... COERCE ...
 
-  Therefore, the state defined in this module in shared by the idealizations
-  of all modules in the key schedule stack and should not be directly accessible
-  to the adversary, even though there is no such access control in this module
-  because each KEF and KDF module will need access to the safety table.
-*)
+  This requires concrete safe/auth/strong/honest functions,
+  used solely for controlling idealization.                        *)
+
 
 // -------------------------------------------------------------------
 // Application configuration
@@ -79,6 +78,7 @@ type ServerCertificateRequest // something that determines this Handshake messag
 request_client_certificate: single_assign ServerCertificateRequest // uses this one, or asks the server; by default Some None.
 
 *)
+
 
 noeq type config = {
     (* Supported versions, ciphersuites, groups, signature algorithms *)
@@ -240,20 +240,21 @@ let ne_default =
 }
 
 // -------------------------------------------------------------------
-//         TLS 1.2 indexing and safety predicates
-// -------------------------------------------------------------------
-
 // Pre Master Secret indexes
+
+// Placeholder for overhaul of 1.2 indexes
 type pmsId = PMS.pms
 assume val strongKEX: pmsId -> Tot bool
 
 // -------------------------------------------------------------------
 // Master Secret indexes and their properties
+
 // CF postv1, move strength predicates --> TLSConstants
 // ``kefAlg is a strong randomness extractor, despite all other kefAlgs'', guarding idealization in KEF
 
-// guarding idealizations for KDF and VerifyData (see PRF.fs)
 assume val strongKEF: kefAlg_t -> Tot bool
+
+// guarding idealizations for KDF and VerifyData (see PRF.fs)
 assume val strongKDF: kdfAlg_t -> Tot bool
 assume val strongVD: vdAlg_t -> Tot bool
 
@@ -322,7 +323,6 @@ val siAuthEncAlg: si:sessionInfo { si.protocol_version = TLS_1p2 &&
                               pvcs si.protocol_version si.cipher_suite } -> Tot aeAlg
 let siAuthEncAlg si = get_aeAlg si.cipher_suite
 
-// Master sectet index
 type msId = // We record the parameters used to derive the master secret;
   | StandardMS : pmsId -> csRands -> kefAlg_t -> msId
             // the pms index, the nonces, and the PMS-PRF algorithm
@@ -334,6 +334,11 @@ type msId = // We record the parameters used to derive the master secret;
 let honestMS = function
   | StandardMS pmsId csr ka -> PMS.honestPMS pmsId && strongKEF ka
   | ExtendedMS pmsId  sh ka -> PMS.honestPMS pmsId && strongKEF ka
+
+
+// ADL Keeping these comments from 0.9 temporarily
+// We don't rely on noPmsId and noMsId anymore; plaintext
+// epochs use a special case in the id type
 
 //CF are we missing a correlation with csr?
 //MK we don't allow leak, so every MS derived from an
@@ -407,13 +412,14 @@ assume val strongAESI: sessionInfo -> Tot bool
 // |  ID13   /    |    \
 // |        /     |     \
 //  --->  esId -> hsId -> asId
-//          \      \
-//           \      --<-- CommonDH.share
-//            \
-//             -<-- PSK.pskid
+//          \
+//           --<-- psk_identifier
 //
 // Index type definitions [1.2]:
+//
 //    pmsId -> msId -> ID12
+//
+// type id = PlaintextID | ID12 msId | ID13 keyId
 
 // Info type carried by hashed log
 // The actual log is ghost but the info is carried in the index
@@ -489,25 +495,16 @@ type log_info (li:logInfo) (h:hashed_log) =
   injective #hashed_log #logInfo #equalBytes #eq_logInfo f /\ f h = li
 
 type pre_esId : Type0 =
-  | ApplicationPSK: i:PSK.pskid -> ha:hash_alg{PSK.compatible_hash i ha} -> pre_esId
-  | ResumptionPSK: i:pre_rmsId -> pre_esId
-  | NoPSK: ha:hash_alg -> pre_esId
+  | ApplicationPSK: info:PSK.pskInfo -> i:PSK.psk_identifier -> pre_esId
+  | ResumptionPSK: info:PSK.pskInfo -> i:pre_rmsId -> pre_esId
 
 and pre_hsId =
-  | HSID_PSK: pre_saltId -> pre_hsId // KEF_PRF idealized
-  | HSID_DHE: pre_saltId -> g:CommonDH.group -> si:CommonDH.share g -> sr:CommonDH.share g -> pre_hsId // KEF_PRF_ODH idealized
+  | HSID_PSK: pre_esId -> pre_hsId
+  | HSID_PSK_DHE: pre_esId -> g:CommonDH.group -> initiator:CommonDH.share g -> responder:CommonDH.share g -> pre_hsId
+  | HSID_DHE: hash_alg -> g:CommonDH.group -> initiator:CommonDH.share g -> responder:CommonDH.share g -> pre_hsId
 
 and pre_asId =
-  | ASID: pre_saltId -> pre_asId
-
-and pre_saltId =
-  | EarlySalt: pre_esId -> pre_saltId
-  | HandshakeSalt: pre_hsId -> pre_saltId
-
-and pre_secretId =
-  | EarlySecretID: pre_esId -> pre_secretId
-  | HandshakeSecretID: pre_hsId -> pre_secretId
-  | ApplicationSecretID: pre_asId -> pre_secretId
+  | ASID: pre_hsId -> pre_asId
 
 and pre_rmsId =
   | RMSID: pre_asId -> logInfo -> hashed_log -> pre_rmsId
@@ -515,16 +512,17 @@ and pre_rmsId =
 and pre_exportId =
   | ExportID: pre_asId -> logInfo -> hashed_log -> pre_exportId
 
-and expandTag =
-  | EarlyTrafficSecret
-  | HandshakeTrafficSecret
-  | ApplicationTrafficSecret
-  | TrafficSecret
+and pre_rekeyId =
+  | RekeyID: pre_asId -> logInfo -> hashed_log -> nat -> pre_rekeyId
 
 and pre_expandId =
-  | ExpandedSecret: pre_secretId -> expandTag -> logInfo -> hashed_log -> pre_expandId
+  | EarlySecretID: pre_esId -> pre_expandId
+  | HandshakeSecretID: pre_hsId -> pre_expandId
+  | ApplicationSecretID: pre_asId -> pre_expandId
+  | RekeySecretID: pre_rekeyId -> pre_expandId
 
 and keyTag =
+  | EarlyTrafficKey
   | EarlyApplicationDataKey
   | HandshakeKey
   | ApplicationDataKey
@@ -544,34 +542,24 @@ and pre_finishedId =
 val esId_hash: pre_esId -> Tot hash_alg
 val hsId_hash: pre_hsId -> Tot hash_alg
 val asId_hash: pre_asId -> Tot hash_alg
-val saltId_hash: pre_saltId -> Tot hash_alg
-val secretId_hash: pre_secretId -> Tot hash_alg
 val rmsId_hash: pre_rmsId -> Tot hash_alg
 val exportId_hash: pre_exportId -> Tot hash_alg
+val rekeyId_hash: pre_rekeyId -> Tot hash_alg
 val expandId_hash: pre_expandId -> Tot hash_alg
 val keyId_hash: pre_keyId -> Tot hash_alg
 val finishedId_hash: pre_finishedId -> Tot hash_alg
 
 let rec esId_hash = function
-  | ApplicationPSK pskid h -> h
-  | ResumptionPSK i -> rmsId_hash i
-  | NoPSK h -> h
+  | ApplicationPSK ctx _ -> PSK.pskInfo_hash ctx
+  | ResumptionPSK _ rmsId -> rmsId_hash rmsId
 
 and hsId_hash = function
-  | HSID_PSK i -> saltId_hash i
-  | HSID_DHE i _ _ _ -> saltId_hash i
+  | HSID_PSK i -> esId_hash i
+  | HSID_DHE h _ _ _ -> h
+  | HSID_PSK_DHE i _ _ _ -> esId_hash i
 
 and asId_hash = function
-  | ASID i -> saltId_hash i
-
-and saltId_hash = function
-  | EarlySalt i -> esId_hash i
-  | HandshakeSalt i -> hsId_hash i
-
-and secretId_hash = function
-  | EarlySecretID i -> esId_hash i
-  | HandshakeSecretID i -> hsId_hash i
-  | ApplicationSecretID i -> asId_hash i
+  | ASID i -> hsId_hash i
 
 and rmsId_hash = function
   | RMSID asId _ _ -> asId_hash asId
@@ -579,112 +567,78 @@ and rmsId_hash = function
 and exportId_hash = function
   | ExportID asId _ _ -> asId_hash asId
 
+and rekeyId_hash = function
+  | RekeyID i _ _ _ -> asId_hash i
+
 and expandId_hash = function
-  | ExpandedSecret i _ _ _ -> secretId_hash i
+  | EarlySecretID es -> esId_hash es
+  | HandshakeSecretID hs -> hsId_hash hs
+  | ApplicationSecretID asId -> asId_hash asId
+  | RekeySecretID (RekeyID asId _ _ _) -> asId_hash asId
 
-and keyId_hash = function
-  | KeyID i _ _ _ _ -> expandId_hash i
+and keyId_hash (KeyID i _ _ _ _) = expandId_hash i
 
-and finishedId_hash = function
-  | FinishedID i _ _ _ _ -> expandId_hash i
+and finishedId_hash (FinishedID i _ _ _ _) = expandId_hash i
 
-type valid_hlen (b:bytes) (h:hash_alg) =
-  length b = Hashing.Spec.tagLen h
+type valid_hlen (b:bytes) (h:hash_alg) = length b = Hashing.Spec.tagLen h
 
-type pre_index =
-| I_ES of pre_esId
-| I_HS of pre_hsId
-| I_AS of pre_asId
-| I_SALT of pre_saltId
-| I_SECRET of pre_secretId
-| I_RMS of pre_rmsId
-| I_EXPORT of pre_exportId
-| I_EXPAND of pre_expandId
-| I_KEY of pre_keyId
-| I_FINISHED of pre_finishedId
+val valid_esId: pre_esId -> GTot Type0
+val valid_hsId: pre_hsId -> GTot Type0
+val valid_asId: pre_asId -> GTot Type0
+val valid_rmsId: pre_rmsId -> GTot Type0
+val valid_exportId: pre_exportId -> GTot Type0
+val valid_rekeyId: pre_rekeyId -> GTot Type0
+val valid_expandId: pre_expandId -> GTot Type0
+val valid_keyId: pre_keyId -> GTot Type0
+val valid_finishedId: pre_finishedId -> GTot Type0
 
-type honest_index (i:pre_index) = bool
+let rec valid_esId = function
+  | ApplicationPSK ctx i -> MR.witnessed (PSK.valid_app_psk ctx i)
+  | ResumptionPSK ctx i -> valid_rmsId i // /\ (MR.witnessed (valid_res_psk ctx i))
+and valid_hsId = function
+  | HSID_PSK i -> valid_esId i
+  | HSID_PSK_DHE i _ _ _ -> valid_esId i
+  | HSID_DHE _ _ _ _ -> True
+and valid_asId = function
+  | ASID i -> valid_hsId i
+and valid_rmsId = function
+  | RMSID i li log -> valid_asId i
+      /\ valid_hlen log (asId_hash i)
+      /\ log_info li log
+and valid_exportId = function
+  | ExportID i li log -> valid_asId i
+      /\ valid_hlen log (asId_hash i)
+      /\ log_info li log
+and valid_rekeyId = function
+  | RekeyID i li log _ -> valid_asId i
+      /\ valid_hlen log (asId_hash i)
+      /\ log_info li log
+and valid_expandId = function
+  | EarlySecretID i -> valid_esId i
+  | HandshakeSecretID i -> valid_hsId i
+  | ApplicationSecretID i -> valid_asId i
+  | RekeySecretID i -> valid_rekeyId i
+and valid_keyId = function
+  | KeyID i tag rw li log ->
+      ((tag == EarlyTrafficKey \/ tag == EarlyApplicationDataKey) ==> rw == Client)
+      /\ valid_hlen log (expandId_hash i)
+      /\ log_info li log
+and valid_finishedId = function
+  | FinishedID i tag rw li log ->
+      ((tag == EarlyFinished \/ tag == LateFinished) ==> rw == Client)
+      /\ valid_hlen log (expandId_hash i)
+      /\ log_info li log
 
-let safe_region:rgn = new_region tls_tables_region
-private type i_safety_log = MM.t safe_region pre_index honest_index (fun _ -> True)
-private type s_table = (if Flags.ideal_KEF then i_safety_log else unit)
+type esId = i:pre_esId{valid_esId i}
+type hsId = i:pre_hsId{valid_hsId i}
+type asId = i:pre_asId{valid_asId i}
+type rmsId = i:pre_rmsId{valid_rmsId i}
+type exportId = i:pre_exportId{valid_exportId i}
+type rekeyId = i:pre_rekeyId{valid_rekeyId i}
+type expandId = i:pre_expandId{valid_expandId i}
+type keyId = i:pre_keyId{valid_keyId i}
+type finishedId = i:pre_finishedId{valid_finishedId i}
 
-let safety_table : s_table =
-  (if Flags.ideal_KEF then
-    MM.alloc #safe_region #pre_index #honest_index #(fun _ -> True)
-  else ())
-
-type registered (i:pre_index) =
-  (if Flags.ideal_KEF then
-    let log : i_safety_log = safety_table in
-    MR.witnessed (MM.defined log i)
-  else True)
-
-type valid (i:pre_index) =
-  (match i with
-  | I_ES i ->
-    (match i with
-    | ApplicationPSK i _ -> PSK.registered_psk i
-    | ResumptionPSK i -> registered (I_RMS i)
-    | NoPSK _ -> True)
-  | I_HS i ->
-    (match i with
-    | HSID_PSK i -> registered (I_SALT i)
-    | HSID_DHE i g si sr -> registered (I_SALT i) /\ CommonDH.registered (|g,si|) /\ CommonDH.registered (|g,sr|))
-  | I_AS i ->
-    (match i with
-    | ASID i -> registered (I_SALT i))
-  | I_SALT i ->
-    (match i with
-    | EarlySalt i -> registered (I_ES i)
-    | HandshakeSalt i -> registered (I_HS i))
-  | I_SECRET i ->
-    (match i with
-    | EarlySecretID i -> registered (I_ES i)
-    | HandshakeSecretID i -> registered (I_HS i)
-    | ApplicationSecretID i -> registered (I_AS i))
-  | I_RMS i ->
-    (match i with
-    | RMSID i _ _ -> registered (I_AS i))
-  | I_EXPORT i ->
-    (match i with
-    | ExportID i _ _ -> registered (I_AS i))
-  | I_EXPAND i ->
-    (match i with
-    | ExpandedSecret i _ _ _ -> registered (I_SECRET i))
-  | I_KEY i ->
-    (match i with
-    | KeyID i _ _ _ _ -> registered (I_EXPAND i))
-  | I_FINISHED i ->
-    (match i with
-    | FinishedID i _ _ _ _ -> registered (I_EXPAND i)))
-
-type index = i:pre_index{valid i}
-
-type safe (i:index) =
-  (if Flags.ideal_KEF then
-    let log : i_safety_log = safety_table in
-    MR.witnessed (MM.contains log i true)
-  else False)
-
-type unsafe (i:index) =
-  (if Flags.ideal_KEF then
-    let log : i_safety_log = safety_table in
-    MR.witnessed (MM.contains log i false)
-  else True)
-
-type esId = i:pre_esId{valid (I_ES i)}
-type hsId = i:pre_hsId{valid (I_HS i)}
-type asId = i:pre_asId{valid (I_AS i)}
-type saltId = i:pre_saltId{valid (I_SALT i)}
-type secretId = i:pre_secretId{valid (I_SECRET i)}
-type rmsId = i:pre_rmsId{valid (I_RMS i)}
-type exportId = i:pre_exportId{valid (I_EXPORT i)}
-type expandId = i:pre_expandId{valid (I_EXPAND i)}
-type keyId = i:pre_keyId{valid (I_KEY i)}
-type finishedId = i:pre_finishedId{valid (I_FINISHED i)}
-
-// Top-level index type for version-agile record keys
 type id =
 | PlaintextID: our_rand:random -> id // For IdNonce
 | ID13: keyId:keyId -> id
@@ -695,6 +649,7 @@ let peerId = function
   | ID12 pv msid kdf ae cr sr rw -> ID12 pv msid kdf ae cr sr (dualRole rw)
   | ID13 (KeyID i tag rw li log) ->
       let kid = KeyID i tag (dualRole rw) li log in
+      assume (valid_keyId kid);
       ID13 kid
 
 val siId: si:sessionInfo{
